

x_j : is
either taking
 x_1 or x_2

Dataset :

x_1	x_2	y
1	0	0
2	1	0
3	1	0
4	2	1
5	3	1

$$\theta_1 = 0, \theta_2 = 0$$

$$\alpha = 0.1$$

$$h(\theta)x = \frac{1}{1+e^{-z}}$$

$$z = \theta^T x$$

$$\frac{\partial}{\partial \theta_j} l(\theta) = \sum_{i=1}^n (y^{(i)} - h(\theta(x^{(i)}))) x_j^{(i)}$$

$$(y' - h(\theta(x')) x_j'$$

$$h(\theta)x = \frac{1}{1+e^{-z}}$$

$$z = \theta^T x$$

$$\theta^T = [0 \ 0]$$

$$\theta^T x' = [0 \ 0] [1 \ 0]$$

Vector.

$$= x_1 \theta_1 + x_2 \theta_2 = 1 \cdot 0 + 0 \cdot 0$$

$$= 0$$

$$h(\theta)x$$

$$h(\theta)x = \frac{1}{1+e^{-0}} = \frac{1}{1+1} = \frac{1}{2}$$

$$(y' - \frac{1}{2}) x_j' = (0 - \frac{1}{2}) \cdot 1 = \boxed{-\frac{1}{2}}$$

$$(y^2 - \frac{1}{2}) x_1^2 = (0 - \frac{1}{2}) 2 = -\frac{1}{2} \times 2 = \boxed{-1}$$

$$(y^3 - \frac{1}{2}) x_1^3 = (0 - \frac{1}{2}) 3 = -\frac{1}{2} \times 3 = \boxed{-\frac{3}{2}}$$

$$(y^4 - \frac{1}{2}) x_1^4 = (1 - \frac{1}{2}) 4 = \frac{1}{2} \times 4 = \boxed{2}$$

$$(y^5 - \frac{1}{2}) x_1^5 = (1 - \frac{1}{2}) 5 = \frac{1}{2} \times 5 = \boxed{\frac{5}{2}}$$

$$\sum_{i=1}^5 (y^i - \frac{1}{2}) x_i = -\frac{1}{2} - 1 - \frac{3}{2} + 2 + \frac{5}{2}$$

$$= -\frac{1}{2} - \frac{3}{2} + \frac{5}{2} - 1 + 2$$

$$= \frac{1}{2} - 1 + 2 = \frac{1}{2} + 1$$

$$= \frac{1+2}{2} = \frac{3}{2}$$

$$\boxed{\theta_1 = 1.50}$$

$$\frac{\partial}{\partial \theta_1} = 1.5$$

$$\theta_1 := \theta_1 + \alpha \frac{\partial}{\partial \theta_1}$$

$$:= 0 + 0.5 \times 0.1 \times 1.5$$

$$\boxed{\theta_1 = 0.15}$$

Iteration
or
h

$$j=2 \quad (y^1 - \frac{1}{2})x_2^1 = (0 - \frac{1}{2})0 = 0$$

$$(y^2 - \frac{1}{2})x_2^2 = (0 - \frac{1}{2})1 = -\frac{1}{2}$$

$$(y^3 - \frac{1}{2})x_2^3 = (0 - \frac{1}{2})1 = -\frac{1}{2}$$

$$(y^4 - \frac{1}{2})x_2^4 = (1 - \frac{1}{2})2 = +1$$

$$(y^5 - \frac{1}{2})x_2^5 = (1 - \frac{1}{2})3 = +\frac{3}{2}$$

$$\frac{\partial l(\theta)}{\partial \theta_2} = 0 - \frac{1}{2} - \frac{1}{2} + 1 + \frac{3}{2} = 0 - 0.5 - 0.5$$

$$= -\frac{1}{2} - \frac{1}{2} + \frac{3}{2} + 1 = \frac{5}{2} = 2.5$$

$$= -\frac{5}{2} = -2.5$$

$$\frac{1}{2} + 1 = \frac{3}{2} = 1.5$$

$$\theta_2 := \theta_2 + \alpha \frac{\partial l}{\partial \theta_2}$$

$$1.2 \quad 0 \quad + 0.1 \times + 2.5 \quad 1.5 = \theta_2 = 0.35$$

$$\boxed{\theta_2 = 0.15}$$